minor: prove pbpsteps preserves satisfiability
- actually a stronger statement is possible, but this is set up for
later when we add non-equivalence preserving steps

examples/pseudo_bool/pb_checkScript.sml
@@ -10,6 +10,8 @@ val _ = numLib.prefer_num();
 (* pbp = pseudo-boolean proof format
   Below, nums represent ConstraintIds, which are 1-indexed (although 0s internally work fine)
 *)
+
+(* A constraint to be added by a cutting planes proof *)
 Datatype:
   constr =
   | Id num              (* Constraints can refer to earlier IDs *)
@@ -39,17 +41,17 @@ Type pbf = ``:pb_constraint spt``;
 Type pbp = ``:pbpstep list``;
 
 (* Computes the LHS term of the slack of a constraint under
-  a partial assignment p (list of literals) *)
+  a partial assignment p (list of literals)
 Definition lslack_def:
   lslack (PBC ls num) p =
   SUM (MAP FST (FILTER (λ(a,b). ¬MEM (negate b) p) ls))
 End
 
 Definition check_contradiction_def:
-  check_contradiction (PBC ls num) =
+  check_contradiction (PBC ls num) = ¬
   let l = lslack (PBC ls num) [] in
     l < num
-End
+End *)
 
 Definition check_polish_def:
   (check_polish fml (Id n) = lookup n fml) ∧
@@ -93,21 +95,23 @@ Definition check_pbpstep_def:
     | SOME c => Cont (insert id c fml) (id+1)
 End
 
+Definition check_pbpsteps_def:
+  (check_pbpsteps [] fml id = Cont fml id) ∧
+  (check_pbpsteps (step::steps) fml id =
+    case check_pbpstep step fml id of
+      Cont fml' id' => check_pbpsteps steps fml' id'
+    | res => res)
+End
+
 (* Copied from satSem: this is the set of pseudoboolean constraints *)
 (* TODO: probably move *)
 Definition values_def:
   values s = {v | ∃n. lookup n s = SOME v}
 End
 
-(* TODO: every constraint is satisfied, maybe rename eval_pbc to satisfies_pbc *)
-Definition satisfies_def:
-  satisfies w pbf ⇔
-  ∀c. c ∈ values pbf ⇒ eval_pbc w c
-End
-
 Theorem check_polish_correct:
   ∀n c w.
-  check_polish fml n = SOME c ∧ satisfies w fml ⇒
+  check_polish fml n = SOME c ∧ satisfies w (values fml) ⇒
   eval_pbc w c
 Proof
   Induct_on`n`>>rw[check_polish_def]
@@ -138,5 +142,153 @@ Proof
     match_mp_tac weaken_thm>>
     metis_tac[])
 QED
+
+Theorem check_polish_compact:
+  ∀n c.
+  (∀c. c ∈ values fml ⇒ compact c) ∧
+  check_polish fml n = SOME c ⇒
+  compact c
+Proof
+  Induct_on`n`>>rw[check_polish_def]
+  >- (
+    (*Id case*)
+    fs[values_def]>>metis_tac[])
+  >- (
+    (* add case *)
+    metis_tac[compact_add])
+ >- (
+    (* multiply case *)
+    metis_tac[compact_multiply])
+  >- (
+    (* divide case TODO: must be changed to ensure compactness(?) *)
+    cheat)
+  >- (
+    (* saturate case TODO: must be changed to ensure compactness *)
+    cheat)
+  >- (
+    (* literal case *)
+    EVAL_TAC)
+  >- (
+    (* weaken case *)
+    cheat)
+QED
+
+Theorem check_contradiction_unsat:
+  check_contradiction c ⇒
+  ¬eval_pbc w c
+Proof
+  Cases_on`c`>>rw[check_contradiction_def,eval_pbc_def,lslack_def]>>
+  CCONTR_TAC>>fs[]>>
+  qmatch_asmsub_abbrev_tac`MAP FST lss`>>
+  `lss = l` by
+    fs[Abbr`lss`,FILTER_EQ_ID,EVERY_MEM,FORALL_PROD]>>
+  rw[]>>
+  `SUM (MAP (eval_term w) l) ≤ SUM (MAP FST l)` by
+      (match_mp_tac SUM_MAP_same_LE>>
+      fs[EVERY_MEM,FORALL_PROD]>>
+      rw[]>>
+      rename1`eval_lit w r`>>
+      assume_tac eval_lit_bool>>
+      fs[])>>
+  fs[]
+QED
+
+(* TODO: copied *)
+Theorem values_delete:
+  values (delete h v) ⊆ values v
+Proof
+  simp[values_def,lookup_delete,SUBSET_DEF]>>
+  metis_tac[]
+QED
+
+Theorem values_insert:
+  C ∈ values (insert n l fml) ⇒ C ∈ values fml ∨ C = l
+Proof
+  fs[values_def,lookup_insert]>>
+  rw[]>>
+  every_case_tac>>fs[]>>
+  metis_tac[]
+QED
+
+Theorem values_insert2:
+  values (insert n l fml) ⊆ l INSERT values fml
+Proof
+  rw[SUBSET_DEF]>>
+  metis_tac[values_insert]
+QED
+
+Theorem values_FOLDL_delete:
+  ∀ls v.
+  values (FOLDL (λa b. delete b a) v ls) ⊆ values v
+Proof
+  Induct>>rw[]>>
+  first_x_assum (qspec_then`delete h v` mp_tac)>>rw[]>>
+  match_mp_tac SUBSET_TRANS>>
+  asm_exists_tac>>simp[]>>
+  simp[values_delete]
+QED
+
+Theorem satisfiable_subset:
+  satisfiable t ∧ s ⊆ t ⇒
+  satisfiable s
+Proof
+  rw[satisfiable_def,SUBSET_DEF,satisfies_def]>>
+  metis_tac[]
+QED
+
+Theorem check_pbpstep_Cont:
+  check_pbpstep step fml id = Cont fml' id' ⇒
+  satisfiable (values fml) ⇒ satisfiable (values fml')
+Proof
+  Cases_on`step`>>fs[check_pbpstep_def]>>
+  every_case_tac
+  >- (
+    (* constraint deletion *)
+    rw[]>>
+    drule satisfiable_subset>>
+    disch_then match_mp_tac>>
+    fs[values_FOLDL_delete])
+  >> (
+    (* check_polish *)
+    rw[]>>
+    drule check_polish_correct>>
+    fs[satisfiable_def,satisfies_def]>>
+    rw[]>>qexists_tac`w`>>
+    rw[]>>
+    drule values_insert >> fs[]>>
+    metis_tac[])
+QED
+
+Theorem check_pbpstep_Unsat:
+  check_pbpstep step fml id = Unsat ⇒
+  ¬ satisfiable (values fml)
+Proof
+  Cases_on`step`>>fs[check_pbpstep_def]>>
+  every_case_tac>>
+  (* check_contradiction *)
+  rw[satisfiable_def,values_def,satisfies_def]>>
+  drule check_contradiction_unsat>>
+  metis_tac[]
+QED
+
+Theorem check_pbpsteps_correct:
+  ∀steps fml id.
+  case check_pbpsteps steps fml id of
+    Cont fml' id' =>
+      satisfiable (values fml) ⇒ satisfiable (values fml')
+  | Unsat =>
+      ¬ satisfiable (values fml)
+  | Fail => T
+Proof
+  Induct>>rw[check_pbpsteps_def]>>
+  every_case_tac>>fs[]
+  >- (
+    drule check_pbpstep_Unsat>>fs[])>>
+  (* two subgoals *)
+  first_x_assum(qspecl_then [`s`,`n`] assume_tac)>>rfs[]>>
+  metis_tac[check_pbpstep_Cont]
+QED
+
+(* TODO: write a parser *)
 
 val _ = export_theory ();
